Derivatives (through B.19)

theories/Environment.v
@@ -11,7 +11,9 @@ From LambdaST Require Import
 Definition env : Set := ident -> option prefix.
 
 Definition subst : ident -> prefix -> env -> env := fun id p n x => if eq_id id x then Some p else n x.
+Arguments subst p n x/.
 Definition union : env -> env -> env := fun n n' x => match n' x with None => n x | Some y => Some y end.
+Arguments union n n' x/.
 
 Definition MapsTo : prefix -> ident -> env -> Prop := fun p x n => n x = Some p.
 Arguments MapsTo/ p x n. (* unfold immediately *)
@@ -19,20 +21,37 @@ Arguments MapsTo/ p x n. (* unfold immediately *)
 Notation "n x |-> p" := (MapsTo p x n) (at level 98).
 
 (* Theorem B.10, part I *)
-Theorem maps_to_unique : forall p x n, MapsTo p x n -> ~exists q, p <> q /\ MapsTo q x n.
+Theorem maps_to_unique_literal : forall p x n,
+  MapsTo p x n ->
+  ~exists q, p <> q /\ MapsTo q x n.
 Proof.
   intros p x n Hp [q [Hpq Hq]]. simpl in *. rewrite Hp in Hq. invert Hq. apply Hpq. reflexivity.
 Qed.
 
-Definition EmptyOn : context -> env -> Prop := fun s n =>
-  Forall (fun x => exists p, (MapsTo p x n) /\ Empty p) (vars_in s).
+Theorem maps_to_unique : forall p1 p2 x n,
+  MapsTo p1 x n ->
+  MapsTo p2 x n ->
+  p1 = p2.
+Proof. intros p1 p2 x n H1 H2. simpl in *. rewrite H1 in H2. invert H2. reflexivity. Qed.
 
-Definition MaximalOn : context -> env -> Prop := fun s n =>
-  Forall (fun x => exists p, (MapsTo p x n) /\ Maximal p) (vars_in s).
+(* Generalization of `emptyOn` and `maximalOn` from the paper *)
+Definition prop_on_item : (prefix -> Prop) -> env -> ident -> Prop :=
+  fun P n x => exists p, MapsTo p x n /\ P p.
+Arguments prop_on_item P n x/.
+
+Definition PropOn : (prefix -> Prop) -> context -> env -> Prop := fun P s n => Forall (prop_on_item P n) (vars_in s).
+Arguments PropOn/ P s n.
+
+Definition EmptyOn := PropOn Empty.
+Arguments EmptyOn/ s n.
+
+Definition MaximalOn := PropOn Maximal.
+Arguments MaximalOn/ s n.
 
 (* TODO: empty/maximal on (free variables in) terms *)
 
 Definition Agree n n' D D' : Prop := (MaximalOn D n <-> MaximalOn D' n') /\ (EmptyOn D n <-> EmptyOn D' n').
+Arguments Agree/ n n' D D'.
 
 Inductive EnvTyped : env -> context -> Prop :=
   | EnvTyEmpty : forall n,
@@ -73,7 +92,22 @@ Proof.
   exists p. split; assumption.
 Qed.
 
-(*
+Lemma prop_on_item_weakening : forall P n n' vs,
+  prop_on_item P n' vs ->
+  prop_on_item P (union n n') vs.
+Proof. intros P n n' vs [p [Hn' Hp]]. exists p. split; [| assumption]. simpl. rewrite Hn'. reflexivity. Qed.
+
+Lemma env_typed_weakening : forall n n' G,
+  EnvTyped n' G ->
+  EnvTyped (union n n') G.
+Proof.
+  intros n n' G H. generalize dependent n.
+  induction H; intros; econstructor;
+  try apply IHEnvTyped1; try apply IHEnvTyped2;
+  [simpl; rewrite H; reflexivity | assumption |].
+  destruct H1; [left | right]; (eapply Forall_impl in H1; [apply H1 | apply prop_on_item_weakening]).
+Qed.
+
 (* Theorem B.11 *)
 Theorem agree_union : forall n n' G G' D D',
   FindReplace D D' G G' ->
@@ -82,6 +116,10 @@ Theorem agree_union : forall n n' G G' D D',
   Agree n n' D D' ->
   EnvTyped (union n n') G'.
 Proof.
-  intros n n' G G' D D' Hhole Hn Hn' HA.
-Qed.
-*)
+  intros n n' G G' D D' Hhole Hn Hn' [HAm HAe].
+  generalize dependent n. generalize dependent n'.
+  induction Hhole; intros.
+  - apply env_typed_weakening. assumption.
+  - invert Hn. constructor.
+    + apply IHHhole; assumption.
+    + Abort.
